\documentclass[10pt, a4paper]{article}
\usepackage[top=80pt, bottom=50pt, left=72pt, right=55pt]{geometry}
\usepackage{enumerate}
\usepackage[fleqn]{amsmath}
\usepackage{graphicx}
\begin{document}
\title{PH-105 Assignment Sheet - 1}
\author{Ashwin P. Paranjape}
\date{}
\maketitle
\begin{enumerate}
\item[4.]{An inertial frame $S'$  moves relative to another frame $S$ with a velocity $v_1 \hat{i} + v_2 \hat{j}$ in such a way that $x$ and $x'$ axes and $y$ and $y'$ axes and $z$ and $z'$ axes are always parallel. Let the time $t=t'=0$ when the origin of the frames are coincident. Find the lorentz transformation relaing the coordinates and time of $S'$ to those in $S$.\\


{\underline {\bf Solution}} : \\
As we know the Lorentz transformation when relative velocity is along x axis, we need to convert the coordinates of the two given frames $S$ and $S'$ to $S_R$ and $S_R'$ respectively. Here the frames $S_R$ and $S_R'$ are rotated frames such that the relative velocity between these frames is along the $x_R$ and $x_R'$ axes. Let $\theta = tan^-1(v_2/v_1)$ and v be the magnitude of velocity vector. Thus angle between $S_R$ and $S$ is $\theta$, $S_R'$ and $S'$ is $\theta$.

To get $S_R$ from $S$, we take take components of $x$ and $y$ axes along $x_R$ and $y_R$. Note that time coordinate does not change due to rotation.
\[x_R = x cos \theta + y sin \theta \]
\[y_R = y cos \theta - x sin \theta \]
\[t_R = t\]

Now to get $x_R'$ and $y_R'$ we use lorentz transformation.

\[x_R'=\gamma ( x_R - vt_R) = \gamma (x cos\theta + y sin\theta - v t)\]
\[y_R' = y_R = y cos \theta - xsin\theta\]
\[t_R'= \gamma (t_R - \frac{v x_R}{c^2}) = t-\frac{v (xcos\theta+ysin\theta)}{c^2}\]

To get $x'$ and $y'$ we use take components of $x_R'$ and $y_R'$ on $x'$ and $y'$
\begin{eqnarray*}
x' &=&x_R' cos \theta - y_R' sin \theta \\&= &\gamma ( x cos \theta + y sin \theta - vt)cos\theta - (ycos\theta -xsin\theta)sin\theta\\
   &= &x(\gamma cos^2 \theta +sin^2 \theta) + y (\gamma sin \theta cos \theta - cos \theta sin \theta)-\gamma v t cos \theta\\
y' &= &y_R' cos \theta + x_R' sin \theta \\
   &=& (ycos\theta - xsin\theta)cos\theta + \gamma (xcos\theta +ysin\theta -vt) sin\theta\\
   &= &(ycos^2\theta - xsin\theta cos\theta)+ \gamma (xcos\theta sin\theta +ysin^2\theta-vt sin\theta)\\
   &= &y(cos^2\theta +\gamma sin^2\theta) + x(\gamma cos\theta sin \theta-cos\theta sin \theta) - \gamma v t sin\theta\\
t' &= &t_R'\\
   &= &\gamma (t - v \frac{x cos \theta + y sin \theta}{c^2})
\end{eqnarray*}
}

\end{enumerate}

\end{document}
